theories/lattice.v
@@ -1,4 +1,4 @@
-Require Export sups infs.
+Require Export lfp gfp.
 
 Set Implicit Arguments.
 Unset Printing Implicit Defensive.
@@ -8,7 +8,36 @@ Set Primitive Projections.
 HB.structure Definition boundedPO := {X of botPO X & topPO X }.
 HB.structure Definition Lattice := {X of joinSemiLattice X & meetSemiLattice X }.
 HB.structure Definition boundedLattice := {X of boundedPO X & Lattice X }.
-HB.structure Definition CompleteLattice := {X of PO X & PO_isup X & PO_iinf X }.
+HB.structure Definition CompleteLattice := {X of supCL X & infCL X }.
+
+HB.saturate dual.
+(* HB.saturate setoid_morphism.type. (* hangs *) *)
+HB.saturate po_morphism.type.
+HB.saturate (forall _, _).           (* void... *)
+
+
+(** ** alternative ways to construct sups *)
+
+(** constructing indexed sups from non-indexed ones *)
+HB.factory Record PO_sup X of PO X := {
+    #[canonical=no] sup: (X -> Prop) -> X;
+    #[canonical=no] sup_spec: forall P: X -> Prop, is_sup P (sup P);
+  }.
+HB.builders Context X of PO_sup X.
+  Definition isup I P (h: I -> X) := sup (image h P).
+  Lemma isup_spec I P h: is_sup (image h P) (@isup I P h).
+  Proof. apply: sup_spec. Qed.
+  HB.instance Definition _ := PO_isup.Build X _ isup_spec.
+HB.end.
+
+(** arbitrary sups from directed and binary ones *)
+HB.factory Record PO_cup_dsup X of PO X & PO_cup X & PO_dsup X := {}.
+HB.builders Context X of PO_cup_dsup X.
+  Definition sup (P: X -> Prop) := dsup (sup_closure P) (@directed_sup_closure _ P).
+  Lemma sup_spec P: is_sup P (sup P).
+  Proof. apply is_sup_closure. exact: dsup_spec. Qed.
+  HB.instance Definition _ := PO_sup.Build X _ sup_spec.
+HB.end.
 
 (** constructing complete lattices from their (indexed) sups  *)
 HB.factory Record CL_isup X of supCL X := {}. 
@@ -21,6 +50,29 @@ HB.builders Context X of CL_isup X.
     eapply sup_spec. reflexivity. by move: H=>/forall_image. 
   Qed.
   HB.instance Definition _ := PO_iinf.Build X _ iinf_spec.
+HB.end.
+
+(** ** alternative ways to construct infs *)
+
+(** constructing indexed infs from non-indexed ones *)
+HB.factory Record PO_inf X of PO X := {
+    #[canonical=no] inf: (X -> Prop) -> X;
+    #[canonical=no] inf_spec: forall P: X -> Prop, is_inf P (inf P);
+  }.
+HB.builders Context X of PO_inf X.
+  Definition iinf I P (h: I -> X) := inf (image h P).
+  Lemma iinf_spec I P h: is_inf (image h P) (@iinf I P h).
+  Proof. apply: inf_spec. Qed.
+  HB.instance Definition _ := PO_iinf.Build X _ iinf_spec.
+HB.end.
+
+(** arbitrary infs from codirected and binary ones *)
+HB.factory Record PO_cap_dinf X of PO X & PO_cap X & PO_dinf X := {}.
+HB.builders Context X of PO_cap_dinf X.
+  Definition inf (P: X -> Prop) := dinf (inf_closure P) (@codirected_inf_closure _ P).
+  Lemma inf_spec P: is_inf P (inf P).
+  Proof. apply is_inf_closure. exact: dinf_spec. Qed.
+  HB.instance Definition _ := PO_inf.Build X _ inf_spec.
 HB.end.
 
 (** constructing complete lattices from their (indexed) infs  *)
@@ -36,4 +88,17 @@ HB.builders Context X of CL_iinf X.
   HB.instance Definition _ := PO_isup.Build X _ isup_spec.
 HB.end.
 
+
+
 (* TODO: modular, distributive, residuated, etc *)
+
+(** ** theory *)
+
+Lemma cuptx {X: boundedLattice.type} (x: X): cup top x ≡ top.
+Proof. apply: antisym; auto with lattice. exact: leq_top. Qed.
+Lemma cupxt {X: boundedLattice.type} (x: X): cup x top ≡ top.
+Proof. by rewrite cupC cuptx. Qed.
+Lemma capbx {X: boundedLattice.type} (x: X): cap bot x ≡ bot.
+Proof. exact: (@cuptx (dual X) x). Qed.
+Lemma capxb {X: boundedLattice.type} (x: X): cap x bot ≡ bot.
+Proof. exact: (@cupxt (dual X)). Qed.
