theories/instances.v
@@ -6,6 +6,29 @@ Unset Printing Implicit Defensive.
 Local Unset Transparent Obligations.
 Set Primitive Projections.
 
+
+(** ** Unit *)
+
+Lemma unit_sup_spec P: is_sup P tt.
+Proof. done. Qed.
+HB.instance Definition _ := PO_sup.Build unit _ unit_sup_spec.
+HB.instance Definition _ := CL_isup.Build unit.
+
+(** ** Booleans *)
+
+Lemma bool_bot_spec: is_sup empty false.
+Proof. done. Qed. 
+Lemma bool_top_spec: is_inf empty true.
+Proof. by case. Qed. 
+Lemma bool_cup_spec b c: is_sup (pair b c) (b || c).
+Proof. rewrite is_sup_pair/=. case; case:b; case:c; cbn; intuition discriminate. Qed. 
+Lemma bool_cap_spec b c: is_inf (pair b c) (b && c).
+Proof. rewrite is_inf_pair/=. case; case:b; case:c; cbn; intuition discriminate. Qed. 
+HB.instance Definition _ := PO_bot.Build bool bool_bot_spec.
+HB.instance Definition _ := PO_top.Build bool bool_top_spec.
+HB.instance Definition _ := PO_cup.Build bool _ bool_cup_spec.
+HB.instance Definition _ := PO_cap.Build bool _ bool_cap_spec.
+
 (** ** natural numbers *)
 
 Lemma po_nat: po_axm Peano.le.
@@ -14,6 +37,15 @@ Proof.
   split. now intros <-. intros. now apply Nat.le_antisymm.
 Qed.
 HB.instance Definition _ := isPO.Build nat po_nat.
+Lemma nat_bot_spec: is_sup empty 0.
+Proof. rewrite is_sup_empty/=. exact: le_0_n. Qed.
+Lemma nat_cup_spec n m: is_sup (pair n m) (max n m).
+Proof. rewrite is_sup_pair/=. exact: Nat.max_lub_iff. Qed.
+Lemma nat_cap_spec n m: is_inf (pair n m) (min n m).
+Proof. rewrite is_inf_pair/=. exact: Nat.min_glb_iff. Qed.
+HB.instance Definition _ := PO_bot.Build nat nat_bot_spec.
+HB.instance Definition _ := PO_cup.Build nat max nat_cup_spec.
+HB.instance Definition _ := PO_cap.Build nat min nat_cap_spec.
 
 (** ** lists *)
 
